wip: substitution using re-association

HigherRankSyntax/HigherRankSyntax/Substitution.lean
@@ -33,11 +33,46 @@ def opluss (γ : Shape) : List Shape → Shape
 
 infixl:30 " ⊕⊕ " => Substitution.opluss
 
-def act' {δ α : Shape} (u : α →ˢ δ) : ∀ βs, Expr ((δ ⊕ α) ⊕⊕ βs) → Expr (δ ⊕⊕ βs)
-| [], .varLeft x ◃ ts => x ◃ (fun ⦃β⦄ z => act' u [β] (ts z))
-| [], .varRight y ◃ ts => act' (fun ⦃β⦄ z => act' u [β] (ts z)) [] (u y)
-| β :: βs, .varLeft x ◃ ts => _
-| β :: βs, .varRight y ◃ ts => .varRight y ◃ (fun ⦃β'⦄ z => act' u (β' :: β :: βs) (ts z))
+@[reducible]
+def Renaming.sum {γ δ θ} (f : γ →ʳ θ) (g : δ →ʳ θ) : γ ⊕ δ →ʳ θ
+| _, .varLeft x => f x
+| _, .varRight x => g x
+
+infix:30 " ⊕ʳ " => Renaming.sum
+
+@[reducible]
+def assocLeft {γ δ θ} : γ ⊕ (δ ⊕ θ) →ʳ (γ ⊕ δ) ⊕ θ :=
+  (.varLeft ∘ʳ .varLeft) ⊕ʳ ((.varLeft ∘ʳ .varRight) ⊕ʳ .varRight)
+
+@[reducible]
+def assocRight {γ δ θ} : (γ ⊕ δ) ⊕ θ →ʳ γ ⊕ (δ ⊕ θ) :=
+  (.varLeft ⊕ʳ (.varRight ∘ʳ .varLeft)) ⊕ʳ (.varRight ∘ʳ .varRight)
+
+lemma reassocLR {γ δ θ} : @assocLeft γ δ θ ∘ʳ @assocRight γ δ θ = 𝟙ʳ := by
+  funext α x
+  obtain (_|(_|_)) := x <;> rfl
+
+lemma reassocRL {γ δ θ} : @assocRight γ δ θ ∘ʳ @assocLeft γ δ θ = 𝟙ʳ := by
+  funext α x
+  -- why doesn't the symmetric obtain work here? obtain ((_|_)|_) := x <;> rfl
+  cases x
+  · rfl
+  · case h.h.varRight z =>
+    cases z
+    · rfl
+    · rfl
+
+-- def act' {δ α : Shape} (u : α →ˢ δ) : ∀ βs, Expr ((δ ⊕ α) ⊕⊕ βs) → Expr (δ ⊕⊕ βs)
+-- | [], .varLeft x ◃ ts => x ◃ (fun ⦃β⦄ z => act' u [β] (ts z))
+-- | [], .varRight y ◃ ts => act' (fun ⦃β⦄ z => act' u [β] (ts z)) [] (u y)
+-- | β :: βs, .varLeft x ◃ ts => _
+-- | β :: βs, .varRight y ◃ ts => .varRight y ◃ (fun ⦃β'⦄ z => act' u (β' :: β :: βs) (ts z))
+
+def act' {α β γ : Shape} (u : β →ˢ α) : Expr ((α ⊕ β) ⊕ γ) → Expr (α ⊕ γ)
+  | .varLeft (.varLeft x) ◃ ts => .varLeft x ◃ (fun ⦃δ⦄ z => ⟦ assocLeft ⟧ʳ act' u (⟦ assocRight ⟧ʳ ts z))
+  | .varLeft (.varRight y) ◃ ts => have A := u y ; sorry
+  | .varRight z ◃ ts => .varRight z ◃ (fun ⦃_⦄ z =>  ⟦ assocLeft ⟧ʳ act' u (⟦ assocRight ⟧ʳ ts z))
+
 
 def act {γ δ} (u : γ →ˢ δ) : Expr γ → Expr δ
   | x ◃ ts => act' (fun ⦃β⦄ y => act (u ⇑ˢ β) (ts y)) [] (u x)
@@ -45,6 +80,6 @@ def act {γ δ} (u : γ →ˢ δ) : Expr γ → Expr δ
 def comp {γ δ θ} (u : γ →ˢ δ) (v : δ →ˢ θ) : γ →ˢ θ
 | β, x => act (v ⇑ˢ β) (u x)
 
-notation:90 g:90 " ∘ˢ " f:90 => Substitution.comp f g
+notation:90 g:90 " ∘ˢ " f:91 => Substitution.comp f g
 
 end Substitution
